arrow-examples/Mux2_1.v
@@ -28,8 +28,9 @@ Section notation.
   Local Open Scope kind_scope.
 
   Definition mux2_1
-    : << ArrowKind.Bit, ArrowKind.Bit, ArrowKind.Bit, Unit >> ~> ArrowKind.Bit :=
-    <[ \ sel a b =>
+    : << Bit, << Bit, Bit >>, Unit >> ~> Bit :=
+    <[ \ sel ab =>
+      let '(a,b) = ab in
       let sel_a = and sel a in
       let inv_sel = not sel in
       let sel_b = and inv_sel b in
@@ -45,15 +46,10 @@ Proof. simply_combinational. Qed.
 
 Require Import Cava.Types.
 Require Import Cava.Netlist.
-
-Definition mux2_1_Interface :=
-   combinationalInterface "mux2_1"
-     [mkPort "s" Signal.Bit; mkPort "a" Signal.Bit; mkPort "b" Signal.Bit]
-     [mkPort "o" Signal.Bit]
-     [].
+Require Import Cava.Signal.
 
 Definition mux2_1_netlist :=
-  makeNetlist mux2_1_Interface (build_netlist (closure_conversion mux2_1)).
+  build_netlist (closure_conversion mux2_1) "mux2_1" ("s", ("a", "b")) "o".
 
 Definition mux2_1_tb_inputs : list (bool * (bool * bool)) :=
  [(false, (false, true));
@@ -69,5 +65,8 @@ Definition mux2_1_tb_expected_outputs : list bool :=
 Goal is_combinational (closure_conversion mux2_1). Proof. simply_combinational. Qed.
 
 Definition mux2_1_tb :=
-  testBench "mux2_1_tb" mux2_1_Interface
-            mux2_1_tb_inputs mux2_1_tb_expected_outputs.
+  testBench "mux2_1_tb"
+   (combinationalInterface "mux2_1"
+     [mkPort "s" Bit; mkPort "a" Bit; mkPort "b" Bit]
+     [mkPort "o" Bit] [])
+  (map (fun '(a,(b,c)) => (a,b,c)) mux2_1_tb_inputs) mux2_1_tb_expected_outputs.
