silveroak-opentitan/aes/Arrow/netlists.v
@@ -23,21 +23,21 @@ From Aes Require Import pkg sbox unrolled_opentitan_cipher.
 Require Import Cava.Types.
 Require Import Cava.Netlist.
 
-Definition sbox_canright_interface
-  := combinationalInterface "sbox_canright"
-     (mkPort "op_i" Kind.Bit, mkPort "data_i" (Kind.Vec Kind.Bit 8))
-     (mkPort "data_o" (Kind.Vec Kind.Bit 8))
-     nil.
+(* Definition sbox_canright_interface *)
+(*   := combinationalInterface "sbox_canright" *)
+(*      (mkPort "op_i" Kind.Bit, mkPort "data_i" (Kind.Vec Kind.Bit 8)) *)
+(*      (mkPort "data_o" (Kind.Vec Kind.Bit 8)) *)
+(*      nil. *)
 
-Definition sbox_canright_netlist :=
-  makeNetlist sbox_canright_interface (build_netlist (closure_conversion (aes_sbox SboxCanright))).
+(* Definition sbox_canright_netlist := *)
+(*   makeNetlist sbox_canright_interface (build_netlist (closure_conversion (aes_sbox SboxCanright))). *)
 
-Definition sbox_lut_interface
-  := combinationalInterface "sbox_lut"
-     (mkPort "op_i" Kind.Bit, mkPort "data_i" (Kind.Vec Kind.Bit 8))
-     (mkPort "data_o" (Kind.Vec Kind.Bit 8))
-     nil.
+(* Definition sbox_lut_interface *)
+(*   := combinationalInterface "sbox_lut" *)
+(*      (mkPort "op_i" Kind.Bit, mkPort "data_i" (Kind.Vec Kind.Bit 8)) *)
+(*      (mkPort "data_o" (Kind.Vec Kind.Bit 8)) *)
+(*      nil. *)
 
-Definition sbox_lut_netlist :=
-  makeNetlist sbox_lut_interface (build_netlist (closure_conversion (aes_sbox SboxLut))).
+(* Definition sbox_lut_netlist := *)
+(*   makeNetlist sbox_lut_interface (build_netlist (closure_conversion (aes_sbox SboxLut))). *)
 
